remove dependency on modified iris

external/iris-4.1.0/iris/base_logic/lib/wsat.v
@@ -11,7 +11,7 @@ Module wsatGS.
   Class wsatGpreS (Σ : gFunctors) : Set := WsatGpreS {
     wsatGpreS_inv : inG Σ (gmap_viewR positive (laterO (iPropO Σ)));
     wsatGpreS_enabled : inG Σ coPset_disjR;
-    wsatGpreS_disabled : inG Σ coPset_disjR;
+    wsatGpreS_disabled : inG Σ (gset_disjR positive);
   }.
 
   Class wsatGS (Σ : gFunctors) : Set := WsatG {
@@ -24,7 +24,7 @@ Module wsatGS.
   Definition wsatΣ : gFunctors :=
     #[GFunctor (gmap_viewRF positive (laterOF idOF));
       GFunctor coPset_disjR;
-      GFunctor coPset_disjR].
+      GFunctor (gset_disjR positive)].
 
   Global Instance subG_wsatΣ {Σ} : subG wsatΣ Σ → wsatGpreS Σ.
   Proof. solve_inG. Qed.
@@ -45,17 +45,15 @@ Definition ownE `{!wsatGS Σ} (E : coPset) : iProp Σ :=
 Global Typeclasses Opaque ownE.
 Global Instance: Params (@ownE) 3 := {}.
 
-Definition ownD `{!wsatGS Σ} (E : coPset) : iProp Σ :=
-  own disabled_name (CoPset E).
+Definition ownD `{!wsatGS Σ} (E : gset positive) : iProp Σ :=
+  own disabled_name (GSet E).
 Global Typeclasses Opaque ownD.
 Global Instance: Params (@ownD) 3 := {}.
 
 Definition wsat `{!wsatGS Σ} : iProp Σ :=
   locked (∃ I : gmap positive (iProp Σ),
     own invariant_name (gmap_view_auth (DfracOwn 1) (invariant_unfold <$> I)) ∗
-    ([∗ map] i ↦ Q ∈ I, (ownI i Q) ∗ (▷ Q ∗ ownD {[i]} ∨ ownE {[i]})) ∗
-    (ownD (⊤ ∖ (gset_to_coPset (dom I))))
-    )%I. 
+    [∗ map] i ↦ Q ∈ I, ▷ Q ∗ ownD {[i]} ∨ ownE {[i]})%I.
 
 Section wsat.
 Context `{!wsatGS Σ}.
@@ -90,12 +88,12 @@ Proof. rewrite ownE_disjoint. iIntros (?); set_solver. Qed.
 Lemma ownD_empty : ⊢ |==> ownD ∅.
 Proof.
   rewrite /bi_emp_valid.
-  by rewrite (own_unit (coPset_disjUR) disabled_name).
+  by rewrite (own_unit (gset_disjUR positive) disabled_name).
 Qed.
 Lemma ownD_op E1 E2 : E1 ## E2 → ownD (E1 ∪ E2) ⊣⊢ ownD E1 ∗ ownD E2.
-Proof. intros. by rewrite /ownD -own_op coPset_disj_union. Qed.
+Proof. intros. by rewrite /ownD -own_op gset_disj_union. Qed.
 Lemma ownD_disjoint E1 E2 : ownD E1 ∗ ownD E2 ⊢ ⌜E1 ## E2⌝.
-Proof. rewrite /ownD -own_op own_valid. by iIntros (?%coPset_disj_valid_op). Qed.
+Proof. rewrite /ownD -own_op own_valid. by iIntros (?%gset_disj_valid_op). Qed.
 Lemma ownD_op' E1 E2 : ⌜E1 ## E2⌝ ∧ ownD (E1 ∪ E2) ⊣⊢ ownD E1 ∗ ownD E2.
 Proof.
   iSplit; [iIntros "[% ?]"; by iApply ownD_op|].
@@ -120,85 +118,23 @@ Qed.
 Lemma ownI_open i P : wsat ∗ ownI i P ∗ ownE {[i]} ⊢ wsat ∗ ▷ P ∗ ownD {[i]}.
 Proof.
   rewrite /ownI /wsat -!lock.
-  iIntros "(Hw & Hi & HiE)". iDestruct "Hw" as (I) "[Hw [HI Hd]]".
+  iIntros "(Hw & Hi & HiE)". iDestruct "Hw" as (I) "[Hw HI]".
   iDestruct (invariant_lookup I i P with "[$]") as (Q ?) "#HPQ".
-  iDestruct (big_sepM_delete _ _ i with "HI") as "[[Ho [[HQ $]|HiE']] HI]"; eauto.
+  iDestruct (big_sepM_delete _ _ i with "HI") as "[[[HQ $]|HiE'] HI]"; eauto.
   - iSplitR "HQ"; last by iNext; iRewrite -"HPQ".
-    iExists I. iFrame "Hw". iFrame "Hd". iApply (big_sepM_delete _ _ i); eauto.
+    iExists I. iFrame "Hw". iApply (big_sepM_delete _ _ i); eauto.
     iFrame "HI"; eauto.
   - iDestruct (ownE_singleton_twice with "[$HiE $HiE']") as %[].
 Qed.
 Lemma ownI_close i P : wsat ∗ ownI i P ∗ ▷ P ∗ ownD {[i]} ⊢ wsat ∗ ownE {[i]}.
 Proof.
   rewrite /ownI /wsat -!lock.
-  iIntros "(Hw & Hi & HP & HiD)". iDestruct "Hw" as (I) "[Hw [HI Hd]]".
+  iIntros "(Hw & Hi & HP & HiD)". iDestruct "Hw" as (I) "[Hw HI]".
   iDestruct (invariant_lookup with "[$]") as (Q ?) "#HPQ".
-  iDestruct (big_sepM_delete _ _ i with "HI") as "[[Ho [[HQ ?]|$]] HI]"; eauto.
+  iDestruct (big_sepM_delete _ _ i with "HI") as "[[[HQ ?]|$] HI]"; eauto.
   - iDestruct (ownD_singleton_twice with "[$]") as %[].
-  - iExists I. iFrame "Hw". iFrame "Hd". iApply (big_sepM_delete _ _ i); eauto.
-    iFrame "HI". iFrame "Ho". iLeft. iFrame "HiD". by iNext; iRewrite "HPQ".
-Qed.
-
-Lemma not_in_dom_to_none {V} (I: gmap positive V) (i: positive)
-  (HIi : i ∉ dom I) : I !! i = None.
-Proof.
-  generalize HIi.
-  rewrite elem_of_dom.
-  intros J.
-  unfold is_Some in J.
-  destruct (I !! i); trivial.
-  exfalso. apply J. exists v. trivial.
-Qed.
-
-Lemma get_fresh {V} (g: gmap positive V) : ∃ x , g !! x = None.
-Proof.
-  exists (fresh (dom g)).
-  assert (fresh (dom g) ∉ dom g) as H.
-  {
-    apply is_fresh.
-  }
-  apply not_in_dom_to_none. trivial.
-Qed.
-
-Lemma not_in_dom {V} (I: gmap positive V) (i: positive) :
-  I !! i = None -> i ∈ (⊤ ∖ (gset_to_coPset (dom I))).
-Proof.
-  intro J. rewrite elem_of_difference.
-  rewrite elem_of_gset_to_coPset.
-  rewrite elem_of_dom.
-  rewrite J. split; trivial. apply elem_of_top. trivial.
-Qed.
-  
-Lemma diff_union (s: coPset) (i: positive) :
-    i ∈ s -> s = (s ∖ {[ i ]}) ∪ {[ i ]}.
-Proof.
-  intro. apply set_eq. intros.  rewrite elem_of_union.
-          rewrite elem_of_difference. rewrite elem_of_singleton.
-          have h : Decision (x = i) by solve_decision. destruct h; intuition.
-          subst i. trivial.
-Qed.
-
-Lemma gmap_dom_coPset_insert {V} (I: gmap positive V) (i: positive) (P: V)
-    : gset_to_coPset (dom (<[i:=P]> I)) = (gset_to_coPset (dom I)) ∪ {[ i ]}.
-Proof.
-  apply set_eq.
-  intro x.
-  rewrite elem_of_gset_to_coPset.
-  rewrite elem_of_dom.
-  rewrite elem_of_union.
-  rewrite elem_of_gset_to_coPset.
-  rewrite elem_of_dom.
-  have h : Decision (i = x) by solve_decision. destruct h.
-  - subst x. rewrite elem_of_singleton. rewrite lookup_insert. intuition.
-  - rewrite lookup_insert_ne; trivial. rewrite elem_of_singleton; trivial.
-        intuition. subst x. contradiction.
-Qed.
-    
-Lemma diff_domm_inserted {V} (I: gmap positive V) (i: positive) (P: V)
-    : (⊤ ∖ gset_to_coPset (dom (<[i:=P]> I)))
-     = (⊤ ∖ gset_to_coPset (dom I) ∖ {[ i ]}).
-Proof.
-  rewrite gmap_dom_coPset_insert. set_solver.
+  - iExists I. iFrame "Hw". iApply (big_sepM_delete _ _ i); eauto.
+    iFrame "HI". iLeft. iFrame "HiD". by iNext; iRewrite "HPQ".
 Qed.
 
 Lemma ownI_alloc φ P :
@@ -206,81 +142,45 @@ Lemma ownI_alloc φ P :
   wsat ∗ ▷ P ==∗ ∃ i, ⌜φ i⌝ ∗ wsat ∗ ownI i P.
 Proof.
   iIntros (Hfresh) "[Hw HP]". rewrite /wsat -!lock.
-  
-  iDestruct "Hw" as (I) "[Hw [HI Hd]]".
-  
-  have is_f := Hfresh (@dom _ (gset positive) (gset_dom) I). 
-  destruct is_f as [i [ni phi]].
-  
-  assert (I !! i = None) as HIi by (apply not_in_dom_to_none; trivial).
-  
-  (*have is_f := get_fresh I.
-  destruct is_f as [i HIi].*)
-  assert (i ∈ (⊤ ∖ gset_to_coPset (dom I))) as in_comp. { apply not_in_dom. trivial. }
-  have du := diff_union _ _ in_comp.
-  rewrite du. 
-  
-  iDestruct (ownD_op with "Hd") as "[Hd HE]". { set_solver. }
-  
-  
-  (*iMod (own_unit (coPset_disjUR) disabled_name) as "HE". 
-  
+  iDestruct "Hw" as (I) "[Hw HI]".
+  iMod (own_unit (gset_disjUR positive) disabled_name) as "HE".
   iMod (own_updateP with "[$]") as "HE".
   { apply (gset_disj_alloc_empty_updateP_strong' (λ i, I !! i = None ∧ φ i)).
     intros E. destruct (Hfresh (E ∪ dom I))
       as (i & [? HIi%not_elem_of_dom]%not_elem_of_union & ?); eauto. }
-  iDestruct "HE" as (X) "[Hi HE]"; iDestruct "Hi" as %(i & -> & HIi & ?).*)
-  
-  
+  iDestruct "HE" as (X) "[Hi HE]"; iDestruct "Hi" as %(i & -> & HIi & ?).
   iMod (own_update with "Hw") as "[Hw HiP]".
   { eapply (gmap_view_alloc _ i DfracDiscarded); last done.
     by rewrite /= lookup_fmap HIi. }
-   iModIntro; iExists i;  iSplit; [done|].
-   rewrite /ownI.
-   iDestruct (bi.persistent_sep_dup with "HiP") as "[HiP HiP2]".
-   iFrame "HiP". 
-  
+  iModIntro; iExists i;  iSplit; [done|]. rewrite /ownI; iFrame "HiP".
   iExists (<[i:=P]>I); iSplitL "Hw".
   { by rewrite fmap_insert. }
-  rewrite diff_domm_inserted. iFrame "Hd".
   iApply (big_sepM_insert _ I); first done.
-  iFrame "HI". iFrame "HiP2". iLeft. by rewrite /ownD; iFrame.
+  iFrame "HI". iLeft. by rewrite /ownD; iFrame.
 Qed.
 
 Lemma ownI_alloc_open φ P :
   (∀ E : gset positive, ∃ i, i ∉ E ∧ φ i) →
   wsat ==∗ ∃ i, ⌜φ i⌝ ∗ (ownE {[i]} -∗ wsat) ∗ ownI i P ∗ ownD {[i]}.
 Proof.
-  iIntros (Hfresh) "Hw". rewrite /wsat -!lock. iDestruct "Hw" as (I) "[Hw [HI Hd]]".
-  
-  have is_f := Hfresh (@dom _ (gset positive) (gset_dom) I).
-  destruct is_f as [i [ni phi]].
-  assert (I !! i = None) as HIi by (apply not_in_dom_to_none; trivial).
-  assert (i ∈ (⊤ ∖ gset_to_coPset (dom I))) as in_comp. { apply not_in_dom. trivial. }
-  have du := diff_union _ _ in_comp.
-  rewrite du.
-  iDestruct (ownD_op with "Hd") as "[Hd HD]". { set_solver. }
-  
+  iIntros (Hfresh) "Hw". rewrite /wsat -!lock. iDestruct "Hw" as (I) "[Hw HI]".
+  iMod (own_unit (gset_disjUR positive) disabled_name) as "HD".
+  iMod (own_updateP with "[$]") as "HD".
+  { apply (gset_disj_alloc_empty_updateP_strong' (λ i, I !! i = None ∧ φ i)).
+    intros E. destruct (Hfresh (E ∪ dom I))
+      as (i & [? HIi%not_elem_of_dom]%not_elem_of_union & ?); eauto. }
+  iDestruct "HD" as (X) "[Hi HD]"; iDestruct "Hi" as %(i & -> & HIi & ?).
   iMod (own_update with "Hw") as "[Hw HiP]".
   { eapply (gmap_view_alloc _ i DfracDiscarded); last done.
     by rewrite /= lookup_fmap HIi. }
-  iModIntro; iExists i;  iSplit; [done|].
-  iDestruct (bi.persistent_sep_dup with "HiP") as "[HiP HiP2]".
-  rewrite /ownI; iFrame "HiP". 
+  iModIntro; iExists i;  iSplit; [done|]. rewrite /ownI; iFrame "HiP".
   rewrite -/(ownD _). iFrame "HD".
   iIntros "HE". iExists (<[i:=P]>I); iSplitL "Hw".
   { by rewrite fmap_insert. }
-  rewrite diff_domm_inserted. iFrame "Hd".
   iApply (big_sepM_insert _ I); first done.
-  iFrame "HI". iFrame "HiP2". by iRight.
+  iFrame "HI". by iRight.
 Qed.
 End wsat.
-
-Lemma copset_diff_empty
-    : (⊤ ∖ gset_to_coPset ∅) = ⊤.
-Proof.
-  set_solver.
-Qed.
 
 (* Allocation of an initial world *)
 Lemma wsat_alloc `{!wsatGpreS Σ} : ⊢ |==> ∃ _ : wsatGS Σ, wsat ∗ ownE ⊤.
@@ -289,10 +189,8 @@ Proof.
   iMod (own_alloc (gmap_view_auth (DfracOwn 1) ∅)) as (γI) "HI";
     first by apply gmap_view_auth_valid.
   iMod (own_alloc (CoPset ⊤)) as (γE) "HE"; first done.
-  iMod (own_alloc (CoPset ⊤)) as (γD) "HD"; first done.
+  iMod (own_alloc (GSet ∅)) as (γD) "HD"; first done.
   iModIntro; iExists (WsatG _ _ γI γE γD).
-  rewrite /wsat /ownE /ownD -lock; iFrame.
-  iExists ∅. rewrite fmap_empty big_opM_empty.
-  rewrite copset_diff_empty.
-  iFrame. 
+  rewrite /wsat /ownE -lock; iFrame.
+  iExists ∅. rewrite fmap_empty big_opM_empty. by iFrame.
 Qed.
