src/guarding/wsat_util.v
@@ -4,188 +4,345 @@ From iris.proofmode Require Import proofmode.
 From iris.base_logic.lib Require Export own.
 From iris.base_logic.lib Require Export wsat.
 From iris.prelude Require Import options.
+Import uPred.
+From iris.algebra Require Import functions.
+
+Require Import guarding.conjunct_own_rule.
 
 Section wsat_util.
 
 Context `{!wsatGS.wsatGS Σ}.
 Implicit Types P : iProp Σ.
 
-Lemma ownI_alloc_and_simultaneous_own_alloc (P : positive -> iProp Σ) `{ing : !inG Σ A} (a: A) :
-  (✓ a) ->
-  wsat ==∗ ∃ i, (▷ P i -∗ wsat) ∗ ownI i (P i) ∗ own i a.
+Lemma own_updateP2 `{i : !inG Σ A} (P : A -> Prop) γ (a: A) :
+    a ~~>: P →
+    own.iRes_singleton γ a ~~>: (λ y : iResUR Σ, ∃ a' : A, y = own.iRes_singleton γ a' ∧ P a').
 Proof.
-  intro valid_a.
-  iIntros "Hw". rewrite /wsat -!lock.
-  iDestruct "Hw" as (I) "[Hw [HI Hd]]".
+    intros aP.
+    apply (discrete_fun_singleton_updateP _ (λ m, ∃ x,
+      m = {[ γ := x ]} ∧ ∃ x', 
+      x = own.inG_unfold x' ∧ ∃ a', 
+      x' = cmra_transport inG_prf a' ∧ P a')); [|naive_solver].
+    apply singleton_updateP', (iso_cmra_updateP' own.inG_fold).
+    { apply own.inG_unfold_fold. }
+    { apply (cmra_morphism_op _). }
+    { apply own.inG_unfold_validN. }
+    by apply cmra_transport_updateP'.
+Qed.
+
+Lemma valN_transport `{i : !inG Σ A} n (a: A) :
+  ✓{n} a →
+  ✓{n} cmra_transport inG_prf a.
+Proof.
+  destruct inG_prf. trivial.
+Qed.
+
+          
+Lemma alloc_ok1 `{i : !inG Σ A} `{j : !inG Σ B} n (mz : iResUR Σ) γ γ' (a': A) (b: B) :
+  (γ' ≠ γ) →
+  (mz (inG_id j) !! γ' = None) →
+  ✓{n} b →
+  ✓{n} (own.iRes_singleton γ a' ⋅? Some mz) →
+  ✓{n} (own.iRes_singleton γ a' ⋅ own.iRes_singleton γ' b ⋅? Some mz).
+Proof.
+  unfold "⋅?". intros ne mznone valb valn.
+  rewrite <- cmra_assoc.
+  setoid_replace (own.iRes_singleton γ' b ⋅ mz) with 
+      (mz ⋅ own.iRes_singleton γ' b) by (apply cmra_comm).
+  rewrite cmra_assoc.
+  rewrite /own.iRes_singleton.
+  unfold validN, cmra_validN. unfold ucmra_cmraR, ucmra_validN, iResUR, discrete_funUR.
+  unfold discrete_fun_validN_instance. intros x.
+  unfold validN, cmra_validN. unfold ucmra_cmraR, ucmra_validN, iResUR, gmapUR.
+  unfold gmap_validN_instance. intros γ2.
+  unfold "⋅", cmra_op, ucmra_op, discrete_fun_op_instance.
+  rewrite lookup_op.
   
-  iMod (own_alloc_cofinite a (dom I)) as "ow". { trivial. }
-  iDestruct "ow" as (i) "[%ni ow]".
+  unfold validN, cmra_validN, ucmra_cmraR, ucmra_validN, iResUR, discrete_funUR,
+      discrete_fun_validN_instance,
+      validN, cmra_validN, ucmra_cmraR, ucmra_validN, iResUR, gmapUR, gmap_validN_instance
+      in valn.
+  unfold own.iRes_singleton in valn.
   
-  assert (I !! i = None) as HIi by (apply not_in_dom_to_none; trivial).
+  have h : Decision (inG_id j = x) by solve_decision. destruct h as [h1|h1].
+   - have h : Decision (γ' = γ2) by solve_decision. destruct h as [h2|h2].
+     + have h : Decision (inG_id i = x) by solve_decision. destruct h as [h3|h3].
+       * rewrite <- h3.
+         rewrite discrete_fun_lookup_singleton.
+         rewrite lookup_op.
+         rewrite lookup_singleton_ne. 2: { subst γ2. symmetry. trivial. }
+         rewrite ucmra_unit_left_id. subst γ2. subst x.
+         rewrite h3. rewrite mznone.
+         rewrite ucmra_unit_left_id.
+         
+         rewrite discrete_fun_lookup_singleton.
+         rewrite lookup_singleton.
+         
+         unfold validN, cmra_validN, optionR, option_validN_instance.
+         rewrite own.inG_unfold_validN.
+         apply valN_transport. trivial.
+       * rewrite lookup_op.
+         rewrite discrete_fun_lookup_singleton_ne; trivial.
+          rewrite lookup_empty. rewrite ucmra_unit_left_id.
+          subst γ2. subst x. rewrite mznone.
+         rewrite ucmra_unit_left_id.
+          rewrite discrete_fun_lookup_singleton.
+          rewrite lookup_singleton.
+
+          unfold validN, cmra_validN, optionR, option_validN_instance.
+          rewrite own.inG_unfold_validN.
+          apply valN_transport. trivial.
+    + rewrite <- h1.
+      rewrite discrete_fun_lookup_singleton.
+      rewrite lookup_singleton_ne; trivial.
+      rewrite ucmra_unit_right_id.
+      apply valn.
+  - rewrite cmra_comm.
+    rewrite discrete_fun_lookup_singleton_ne; trivial.
+    rewrite lookup_empty.
+    rewrite ucmra_unit_left_id.
+    apply valn.
+Qed.
+   
+Lemma alloc_ok2 `{i : !inG Σ A} `{j : !inG Σ B} n γ γ' (a': A) (b: B) :
+  (γ' ≠ γ) →
+  ✓{n} b →
+  ✓{n} (own.iRes_singleton γ a' ⋅? None) →
+  ✓{n} (own.iRes_singleton γ a' ⋅ own.iRes_singleton γ' b ⋅? None).
+Proof.
+  unfold "⋅?". intros ne valb valn.
+  rewrite /own.iRes_singleton.
+  unfold validN, cmra_validN. unfold ucmra_cmraR, ucmra_validN, iResUR, discrete_funUR.
+  unfold discrete_fun_validN_instance. intros x.
+  unfold validN, cmra_validN. unfold ucmra_cmraR, ucmra_validN, iResUR, gmapUR.
+  unfold gmap_validN_instance. intros γ2.
+  unfold "⋅", cmra_op, ucmra_op, discrete_fun_op_instance.
+  rewrite lookup_op.
   
-  assert (i ∈ (⊤ ∖ gset_to_coPset (dom I))) as in_comp. { apply not_in_dom. trivial. }
-  have du := diff_union _ _ in_comp.
-  rewrite du.
+  unfold validN, cmra_validN, ucmra_cmraR, ucmra_validN, iResUR, discrete_funUR,
+      discrete_fun_validN_instance,
+      validN, cmra_validN, ucmra_cmraR, ucmra_validN, iResUR, gmapUR, gmap_validN_instance
+      in valn.
+  unfold own.iRes_singleton in valn.
   
-  iDestruct (ownD_op with "Hd") as "[Hd HE]". { set_solver. }
-  
+  have h : Decision (inG_id j = x) by solve_decision. destruct h as [h1|h1].
+   - have h : Decision (γ' = γ2) by solve_decision. destruct h as [h2|h2].
+     + have h : Decision (inG_id i = x) by solve_decision. destruct h as [h3|h3].
+       * rewrite <- h3.
+         rewrite discrete_fun_lookup_singleton.
+         rewrite lookup_singleton_ne. 2: { subst γ2. symmetry. trivial. }
+         rewrite ucmra_unit_left_id.
+         
+         subst x. rewrite h3.
+         rewrite discrete_fun_lookup_singleton.
+         subst γ2. rewrite lookup_singleton.
+         
+         unfold validN, cmra_validN, optionR, option_validN_instance.
+         rewrite own.inG_unfold_validN.
+         apply valN_transport. trivial.
+       * rewrite discrete_fun_lookup_singleton_ne; trivial.
+          rewrite lookup_empty. rewrite ucmra_unit_left_id.
+          rewrite <- h1.
+          rewrite discrete_fun_lookup_singleton.
+          subst γ2. rewrite lookup_singleton.
+          
+          unfold validN, cmra_validN, optionR, option_validN_instance.
+          rewrite own.inG_unfold_validN.
+          apply valN_transport. trivial.
+    + rewrite <- h1.
+      rewrite discrete_fun_lookup_singleton.
+      rewrite lookup_singleton_ne; trivial.
+      rewrite ucmra_unit_right_id.
+      apply valn.
+  - rewrite cmra_comm.
+    rewrite discrete_fun_lookup_singleton_ne; trivial.
+    rewrite lookup_empty.
+    rewrite ucmra_unit_left_id.
+    apply valn.
+Qed.
+          
+Lemma updates_inf_1 `{i : !inG Σ A} `{j : !inG Σ B} (mz : iResUR Σ) (P : A → gname → Prop) γ (a: A) :
+  (∀ (n : nat) (mz : option A) (N : gname → Prop),
+           ✓{n} (a ⋅? mz)
+           → pred_finite N → ∃ (y : A) (γ' : gname), P y γ' ∧ ✓{n} (y ⋅? mz) ∧ ¬ N γ') →
+  a ~~>: (λ a0 : A, ∃ γ' : gname, P a0 γ' ∧ mz (inG_id j) !! γ' = None ∧ γ' ≠ γ).
+Proof.
+  unfold "~~>:". intros Hx n mz0 valn.
+  assert (pred_finite (λ γ' : gname, mz (inG_id j) !! γ' ≠ None ∨ γ' = γ)) as X.
+  {
+    assert (set_finite (dom (mz (inG_id j) : gmap _ _))) as X. { apply dom_finite. }
+    unfold set_finite, pred_finite in X. destruct X as [xs X].
+    unfold pred_finite.
+    exists (γ :: xs).
+    intros x cond.
+    destruct cond as [cond|cond].
+    - rewrite elem_of_cons. right. apply X.
+      rewrite elem_of_dom.
+      destruct (mz (inG_id j) !! x) eqn:ee.
+      + rewrite ee. trivial.
+      + contradiction.
+    - rewrite elem_of_cons. left. trivial.
+  }
+  have t := Hx n mz0 (λ γ', mz (inG_id j) !! γ' ≠ None ∨ γ' = γ) valn X.
+  destruct t as [y [γ' [t [u v]]]].
+  exists y. split; trivial. exists γ'. split; trivial.
+  split.
+  + destruct (mz (inG_id j) !! γ') eqn:ee.
+    - exfalso. apply v. left. intro. discriminate.
+    - trivial.
+  + intuition.
+Qed.
+
+Lemma updates_inf_2 `{i : !inG Σ A} (P : A → gname → Prop) γ (a: A) :
+  (∀ (n : nat) (mz : option A) (N : gname → Prop),
+           ✓{n} (a ⋅? mz)
+           → pred_finite N → ∃ (y : A) (γ' : gname), P y γ' ∧ ✓{n} (y ⋅? mz) ∧ ¬ N γ') →
+  a ~~>: (λ a0 : A, ∃ γ' : gname, P a0 γ' ∧ γ' ≠ γ).
+Proof.
+  unfold "~~>:". intros Hx n mz valn.
+  assert (pred_finite (λ γ' : gname, γ' = γ)) as X.
+  {
+    unfold pred_finite. exists (γ :: nil).
+    intros x. intro eq. subst x. rewrite elem_of_cons. left; trivial.
+  }
+  have t := Hx n mz (λ γ', γ' = γ) valn X.
+  destruct t as [y [γ' [t [u v]]]].
+  exists y. split; trivial. exists γ'. split; trivial.
+Qed.
+
+Lemma own_updateP_extra `{i : !inG Σ A} `{j : !inG Σ B} (P : A → gname → Prop) γ (a : A) (b : B) :
+    (∀ (n : nat) (mz : option A) (N : gname → Prop) , ✓{n} (a ⋅? mz) → pred_finite N → ∃ (y: A) (γ': gname), P y γ' ∧ ✓{n} (y ⋅? mz) ∧ ¬ N γ') →
+    (✓ b) →
+    own γ a ⊢ |==> ∃ a' γ', ⌜P a' γ'⌝ ∗ own γ a' ∗ own γ' b.
+Proof using H Σ.
+  intros Hupd Hvalb. rewrite !own.own_eq.
+  rewrite -(bupd_mono (∃ m,
+    ⌜ ∃ a' γ', m = (own.iRes_singleton γ a' ⋅ own.iRes_singleton γ' b) ∧ P a' γ' ⌝ ∧ uPred_ownM m)%I).
+  - apply bupd_ownM_updateP. unfold "~~>:". intros n mz Hvaln.
+    destruct mz as [mz|].
+      + enough (a ~~>: (λ a : A, ∃ γ' : gname, P a γ' ∧ mz (inG_id j) !! γ' = None ∧ γ' ≠ γ)) as X.
+        {
+          have t := @own_updateP2 A i (λ a, ∃ γ', P a γ' ∧ mz (inG_id j) !! γ' = None ∧ γ' ≠ γ) γ a X.
+          unfold "~~>:" in t.
+          have s := t n (Some mz) Hvaln.
+          destruct s as [y [[a' [oa [γ' [s [mzn ne]]]]] q]].
+          exists (y ⋅ own.iRes_singleton γ' b). split.
+          { exists a'. exists γ'. rewrite oa. split; trivial. }
+          rewrite oa. rewrite oa in q. apply alloc_ok1; trivial.
+          apply cmra_valid_validN. trivial.
+        }
+        {
+          apply updates_inf_1; trivial.
+        }
+      + enough (a ~~>: (λ a : A, ∃ γ' : gname, P a γ' ∧ γ' ≠ γ)) as X.
+        {
+          have t := @own_updateP2 A i (λ a, ∃ γ', P a γ' ∧ γ' ≠ γ) γ a X.
+          unfold "~~>:" in t.
+          have s := t n None Hvaln.
+          destruct s as [y [[a' [oa [γ' [s ne]]]] q]].
+          exists (y ⋅ own.iRes_singleton γ' b). split.
+          { exists a'. exists γ'. rewrite oa. split; trivial. }
+          rewrite oa. rewrite oa in q. apply alloc_ok2; trivial.
+          apply cmra_valid_validN. trivial.
+        }
+        {
+          apply updates_inf_2; trivial.
+        }
+   - apply exist_elim=> m.
+      iIntros "[%s t]".
+      destruct s as [a' [γ' [s p]]].
+      iExists a'. iExists γ'. rewrite s.
+      iSplit. { iPureIntro. trivial. }
+      unfold own.own_def.
+      rewrite ownM_op. iFrame.
+Qed.
+
+Lemma ownI_alloc φ P :
+  (∀ E : gset positive, ∃ i, i ∉ E ∧ φ i) →
+  wsat ∗ ▷ P ==∗ ∃ i, ⌜φ i⌝ ∗ wsat ∗ ownI i P.
+Proof. 
+  iIntros (Hfresh) "[Hw HP]". rewrite /wsat -!lock.
+  iDestruct "Hw" as (I) "[Hw HI]".
+  iMod (own_unit (gset_disjUR positive) wsat.wsatGS.disabled_name) as "HE".
+  iMod (own_updateP with "[$]") as "HE".
+  { apply (gset_disj_alloc_empty_updateP_strong' (λ i, I !! i = None ∧ φ i)).
+    intros E. destruct (Hfresh (E ∪ dom I))
+      as (i & [? HIi%not_elem_of_dom]%not_elem_of_union & ?); eauto. }
+  iDestruct "HE" as (X) "[Hi HE]"; iDestruct "Hi" as %(i & -> & HIi & ?).
   iMod (own_update with "Hw") as "[Hw HiP]".
   { eapply (gmap_view_alloc _ i DfracDiscarded); last done.
     by rewrite /= lookup_fmap HIi. }
-  
-  iModIntro. iExists i.
-  
-  rewrite /ownI.
-  iDestruct (bi.persistent_sep_dup with "HiP") as "[HiP HiP2]".
-  iFrame "HiP". iFrame "ow".
-  iIntros "laterp".
-  iExists (<[i:=P i]>I); iSplitL "Hw".
+  iModIntro; iExists i;  iSplit; [done|]. rewrite /ownI; iFrame "HiP".
+  iExists (<[i:=P]>I); iSplitL "Hw".
   { by rewrite fmap_insert. }
-  
-  rewrite diff_domm_inserted. iFrame "Hd".
-  
   iApply (big_sepM_insert _ I); first done.
-  iFrame "HI". iFrame "HiP2". iLeft. by rewrite /ownD; iFrame.
+  iFrame "HI". iLeft. by rewrite /ownD; iFrame.
 Qed.
 
-Lemma ownI_alloc_and_simultaneous_own_alloc_ns (P : positive -> iProp Σ) `{ing : !inG Σ A} (a:A) (from: coPset) (inf: ¬set_finite from) :
+Lemma ownI_alloc_and_simultaneous_own_alloc_ns (P : positive -> iProp Σ) `{ing : !inG Σ A} (a:A) (from: coPset) (inf: set_infinite from) :
   (✓ a) ->
   wsat ==∗ ∃ i, ⌜ i ∈ from ⌝ ∗ (▷ P i -∗ wsat) ∗ ownI i (P i) ∗ own i a.
 Proof.
   intro valid_a.
   iIntros "Hw". rewrite /wsat -!lock.
-  iDestruct "Hw" as (I) "[Hw [HI Hd]]".
+  iDestruct "Hw" as (I) "[Hw HI]".
   
-  iMod (own_alloc_strong a (λ i , i ∉ dom I ∧ i ∈ from)) as "ow".
+  iMod (own_unit (gset_disjUR positive) wsat.wsatGS.disabled_name) as "HE".
+  
+  iMod (own_updateP_extra (λ a i, (a = GSet {[i]}) ∧ I !! i = None ∧ i ∈ from) wsat.wsatGS.disabled_name ε a  with "[$]") as "HE".
   {
-    unfold pred_infinite.
-    intro xs.
-    assert (set_infinite (from ∖ (gset_to_coPset (dom I)) ∖ list_to_set xs)) as infi.
-    - apply difference_infinite.
-      + apply difference_infinite.
-        * rewrite coPset_infinite_finite. trivial.
-        * apply gset_to_coPset_finite.
-      + apply list_to_set_finite.
-    - exists (coPpick (from ∖ (gset_to_coPset (dom I)) ∖ list_to_set xs)).
-      assert (
-          (coPpick (from ∖ (gset_to_coPset (dom I)) ∖ list_to_set xs))
-          ∈
-          (from ∖ gset_to_coPset (dom I) ∖ list_to_set xs)
-      ) as IN. { apply coPpick_elem_of. rewrite <- coPset_infinite_finite. trivial. }
-      generalize IN.
-      rewrite elem_of_difference.
-      rewrite elem_of_difference.
-      rewrite elem_of_list_to_set.
-      rewrite elem_of_gset_to_coPset.
-      rewrite elem_of_dom.
-      intuition.
+    intros n mz N val_mz finiteN.
+    assert (set_finite (dom I)) as sFin. { apply dom_finite. }
+    unfold pred_finite in finiteN. destruct finiteN as [xs finiteN].
+    unfold set_infinite, pred_infinite in inf.
+    unfold set_finite, pred_finite in sFin.
+    destruct sFin as [xs2 sFin].
+    
+    destruct mz as [mz|].
+    + destruct mz as [mz|].
+      * assert (set_finite mz) as mzFin. { apply fin_set_finite. }
+        unfold set_finite, pred_finite in mzFin.
+        destruct mzFin as [xs3 mzFin].
+    
+        have inf2 := inf (xs ++ xs2 ++ xs3). destruct inf2 as [x [x_in_from x_not_in_xs]].
+        rewrite not_elem_of_app in x_not_in_xs.
+        rewrite not_elem_of_app in x_not_in_xs.
+        destruct x_not_in_xs as [x_not_in_xs [x_not_in_xs2 x_not_in_xs3]].
+        exists (GSet {[x]}).
+        exists x. split; trivial.
+        - split; trivial. split; trivial.
+          rewrite <- not_elem_of_dom. intro x_in_dom. apply x_not_in_xs2. apply sFin. trivial.
+        - split; trivial.
+          ++ unfold "⋅?".  generalize n. rewrite <- cmra_valid_validN.
+              rewrite gset_disj_valid_op. rewrite disjoint_singleton_l.
+              intro xmz. apply x_not_in_xs3. apply mzFin. trivial.
+          ++ intro Nx. apply x_not_in_xs. apply finiteN. trivial.
+     * unfold "⋅?" in val_mz. rewrite ucmra_unit_left_id in val_mz.
+        unfold validN, cmra_validN, gset_disjR, discrete_validN_instance, valid, gset_disj_valid_instance in val_mz. contradiction.
+    + have inf2 := inf (xs ++ xs2). destruct inf2 as [x [x_in_from x_not_in_xs]].
+        rewrite not_elem_of_app in x_not_in_xs.
+        destruct x_not_in_xs as [x_not_in_xs x_not_in_xs2].
+        exists (GSet {[x]}).
+        exists x. split; trivial.
+        - split; trivial. split; trivial.
+          rewrite <- not_elem_of_dom. intro x_in_dom. apply x_not_in_xs2. apply sFin. trivial.
+        - split; trivial.
+          intro Nx. apply x_not_in_xs. apply finiteN. trivial.
   }
   { trivial. }
   
-  iDestruct "ow" as (i) "[%ni ow]".
-  destruct ni as [ni in_from].
-  
-  assert (I !! i = None) as HIi by (apply not_in_dom_to_none; trivial).
-  
-  assert (i ∈ (⊤ ∖ gset_to_coPset (dom I))) as in_comp. { apply not_in_dom. trivial. }
-  have du := diff_union _ _ in_comp.
-  rewrite du.
-  
-  iDestruct (ownD_op with "Hd") as "[Hd HE]". { set_solver. }
+  iDestruct "HE" as (X i) "[[%Xi [%HIi %gfrom]] [Hi HE]]".
   
   iMod (own_update with "Hw") as "[Hw HiP]".
   { eapply (gmap_view_alloc _ i DfracDiscarded); last done.
     by rewrite /= lookup_fmap HIi. }
-  
-  iModIntro. iExists i.
-  
-  rewrite /ownI.
-  iDestruct (bi.persistent_sep_dup with "HiP") as "[HiP HiP2]".
-  iFrame "HiP". iFrame "ow".
-  iSplitL "". { iPureIntro. trivial. }
-  iIntros "laterp".
+  iModIntro; iExists i;  iSplit; [done|]. rewrite /ownI; iFrame "HiP".
+  iFrame.
+  iIntros "latP".
   iExists (<[i:=P i]>I); iSplitL "Hw".
   { by rewrite fmap_insert. }
-  
-  rewrite diff_domm_inserted. iFrame "Hd".
-  
   iApply (big_sepM_insert _ I); first done.
-  iFrame "HI". iFrame "HiP2". iLeft. by rewrite /ownD; iFrame.
-Qed. 
-
-(*
-Lemma ownI_alloc_open_and_simultaneous_own_alloc (P : positive -> iProp Σ) `{ing : !inG Σ A} (a: A) :
-  (✓ a) ->
-  wsat ==∗ ∃ i, (ownE {[i]} -∗ wsat) ∗ ownI i (P i) ∗ ownD {[i]} ∗ own i a.
-Proof.
-  iIntros (valid_a) "Hw". rewrite /wsat -!lock. iDestruct "Hw" as (I) "[Hw [HI Hd]]".
-  
-  iMod (own_alloc_cofinite a (dom _ I)) as "ow". { trivial. }
-  iDestruct "ow" as (i) "[%ni ow]".
-  
-  (*have is_f := Hfresh (@dom _ (gset positive) (gset_dom) I).
-  destruct is_f as [i [ni phi]].*)
-  assert (I !! i = None) as HIi by (apply not_in_dom_to_none; trivial).
-  assert (i ∈ (⊤ ∖ gmap_dom_coPset I)) as in_comp. { apply not_in_dom. trivial. }
-  have du := diff_union _ _ in_comp.
-  rewrite du.
-  iDestruct (ownD_op with "Hd") as "[Hd HD]". { set_solver. }
-  
-  iMod (own_update with "Hw") as "[Hw HiP]".
-  { eapply (gmap_view_alloc _ i DfracDiscarded); last done.
-    by rewrite /= lookup_fmap HIi. }
-  iModIntro. iExists i.
-  iDestruct (bi.persistent_sep_dup with "HiP") as "[HiP HiP2]".
-  rewrite /ownI; iFrame "HiP".
-  rewrite -/(ownD _). iFrame "HD". iFrame "ow".
-  iIntros "HE". iExists (<[i:=P i]>I); iSplitL "Hw".
-  { by rewrite fmap_insert. }
-  
-  rewrite diff_domm_inserted. iFrame "Hd".
-  
-  iApply (big_sepM_insert _ I); first done.
-  iFrame "HI". iFrame "HiP2". by iRight.
-Qed.
-*)
-
-Lemma ownI_alloc_open_or_alloc i :
-  ⊢ wsat ∗ ownE {[i]} ==∗ ∃ P , wsat ∗ ownD {[i]} ∗ ownI i P ∗ ▷ P.
-Proof.
-  rewrite /ownI /wsat -!lock.
-  iIntros "(Hw & HiE)". iDestruct "Hw" as (I) "[Hw [HI Hd]]".
-  destruct (I !! i) eqn:HIi.
-  + (* case 1: invariant exists; open it *)
-    iDestruct (big_sepM_delete _ _ i with "HI") as "[[Ho [[HQ $]|HiE']] HI]"; eauto.
-    - iExists u. iFrame "HQ". rewrite /ownI.
-      iDestruct (bi.persistent_sep_dup with "Ho") as "[Ho1 Ho2]".
-      iFrame "Ho1".
-      iExists I. iFrame "Hw". iFrame "Hd". iApply (big_sepM_delete _ _ i); eauto.
-      iFrame "HI"; eauto.
-    - iDestruct (ownE_singleton_twice with "[$HiE $HiE']") as %[].
-  + (* case 2: invariant doesn't exist; alloc a new one *)
-    iExists ((True)%I : iProp Σ).
-    assert (i ∈ (⊤ ∖ gset_to_coPset (dom I))) as in_comp. { apply not_in_dom. trivial. }
-
-    have du := diff_union _ _ in_comp.
-    rewrite du.
-    iDestruct (ownD_op with "Hd") as "[Hd HD]". { set_solver. }
-
-    iMod (own_update with "Hw") as "[Hw HiP]".
-    { eapply (gmap_view_alloc _ i DfracDiscarded); last done.
-      by rewrite /= lookup_fmap HIi. }
-    iModIntro.
-    iFrame "HD".
-      iDestruct (bi.persistent_sep_dup with "HiP") as "[HiP1 HiP2]".
-    iFrame "HiP1".
-    
-    iSplitL.
-    * iExists (<[i:= ((True)%I : iProp Σ)]>I); iSplitL "Hw".
-      { by rewrite fmap_insert. }
-      rewrite diff_domm_inserted. iFrame "Hd".
-
-      iApply (big_sepM_insert _ I); first done.
-      iFrame "HI". rewrite /ownI. iFrame "HiP2". by iRight.
-    * iModIntro. done.
+  iFrame "HI". iLeft. iFrame. rewrite /ownD. rewrite Xi. iFrame.
 Qed.
 
 End wsat_util.
